# Interlude: proof by induction

## Exercise 4 (example)

### Inducting on lists

Here's the inductive definition of a list again for reference. Each list `l` is either
- The empty list `l ≡ nil`
- An element `x` followed by the remainder `xs` of the list. So `l ≡ x : xs`

Now to prove a proposition `P` holds for all lists `l`, we need only show:
- `P(nil)` is true
- For any `x` and any `xs`, if `P(xs)` is true, then `P(x:xs)` is true.

These cases serve as the base case and inductive step respectively.

If we have proofs of these two cases, we can imagine constructing a proof for any given list `l ≡ [x_1, x_2, ... x_n]`.
We can express `l ≡ x_1 : (x_2 : (... (x_n : nil))... ) ≡ x_1 : x_2 : ... x_n : nil` and construct a proof of `P(l)` by
chaining together the proof of `P(nil)` and n copies of the proof of `P(xs) ⇒ P(x:xs)`.

### An example

Opposite is a proof by induction on lists, that if all elements of a list are even, then their sum is even.

We haven't defined addition, but we will use it here and rely only on the following property: if `x` and `y` are both
even, then `x + y` is even.

The sum of a list is defined inductively:
- If `l ≡ nil` then `sum(l) ≡ 0`
- If `l ≡ x : xs` then `sum(l) = x + sum(xs)`
